backend/Asmgenproof_comp.v
@@ -3121,29 +3121,19 @@ Proof.
     split. eapply MU.
     split. eapply MU.
     split. split. eapply MU. clear MU.
-      destruct MTCH as [_ [_ [PG [_ [GF [SMV WD]]]]]].
       split. apply effstep_corestep in H.
-             eapply mem_respects_readonly_forward'. eassumption.
+             eapply mem_respects_readonly_fwd. eassumption.
              eapply corestep_fwd; eassumption.
-             eapply mach_coop_readonly. apply H.
-         intros b GB. apply GF in GB. eapply SMV.
-         destruct (frgnSrc _ WD _ GB) as [bb [d [Frgn FTgt]]]. eapply foreign_DomRng; eassumption.
-      assert(G2: forall b, isGlobalBlock tge b = true -> Mem.valid_block m2 b).
-         rewrite <- (genvs_domain_eq_isGlobal _ _ GDE_lemma).
-         intros b GB. eapply SMV.
-         apply (meminj_preserves_globals_isGlobalBlock _ _ PG) in GB. 
-         eapply as_inj_DomRng; eassumption.
+             eapply corestep_rdonly; eassumption.
       destruct CSTgt as [CS2 | [_ CS2]].
       apply effstep_plus_corestep_plus in CS2.
-             eapply mem_respects_readonly_forward'. eassumption.
+             eapply mem_respects_readonly_fwd. eassumption.
              eapply corestep_plus_fwd; eassumption.
-             eapply SM_simulation.CS2_RDO_plus; try eassumption.
-             apply asm_coop_readonly. 
+             eapply corestep_plus_rdonly. eassumption. 
       apply effstep_star_corestep_star in CS2.
-             eapply mem_respects_readonly_forward'. eassumption.
+             eapply mem_respects_readonly_fwd. eassumption.
              eapply corestep_star_fwd; eassumption.
-             eapply SM_simulation.CS2_RDO_star; try eassumption.
-             apply asm_coop_readonly. 
+             eapply corestep_star_rdonly. eassumption. 
     (*split. eapply MU. *)
     exists U2. split. trivial. eapply MU. }
 Qed.
