backend/CleanupLabelsproof_comp.v
@@ -1997,28 +1997,20 @@ eapply lt_state_wf.
     split.
     { split; trivial.
       split. apply MU'. clear MU'.
-      destruct MTCH as [_ [_ [PG [_ [GF [SMV [WD _]]]]]]].
       split.
       apply effstep_corestep in H.
-             eapply mem_respects_readonly_forward'. eassumption.
+             eapply mem_respects_readonly_fwd. eassumption.
              eapply corestep_fwd; eassumption.
-             eapply linear_coop_readonly; try eassumption. apply H.
-         intros b GB. apply GF in GB. eapply SMV.
-         destruct (frgnSrc _ WD _ GB) as [bb [d [Frgn FTgt]]]. eapply foreign_DomRng; eassumption.
-     assert(G2: forall b, isGlobalBlock tge b = true -> Mem.valid_block m2 b).
-         rewrite <- (genvs_domain_eq_isGlobal _ _ GDE_lemma).
-         intros b GB. eapply SMV.
-         apply (meminj_preserves_globals_isGlobalBlock _ _ PG) in GB. 
-         eapply as_inj_DomRng; eassumption.
+             eapply corestep_rdonly; eassumption.
       destruct CS' as [CS2 | [_ CS2]]. 
         apply effstep_plus_corestep_plus in CS2.
-             eapply mem_respects_readonly_forward'. eassumption.
+             eapply mem_respects_readonly_fwd. eassumption.
              eapply corestep_plus_fwd; eassumption.
-             eapply SM_simulation.CS2_RDO_plus; try eassumption. apply linear_coop_readonly.
-        apply effstep_star_corestep_star in CS2.
-             eapply mem_respects_readonly_forward'. eassumption.
+             eapply corestep_plus_rdonly. eassumption. 
+      apply effstep_star_corestep_star in CS2.
+             eapply mem_respects_readonly_fwd. eassumption.
              eapply corestep_star_fwd; eassumption.
-             eapply SM_simulation.CS2_RDO_star; try eassumption. apply linear_coop_readonly.
+             eapply corestep_star_rdonly. eassumption. 
     }
     exists U2.
     split. destruct CS'. 
