backend/Constpropproof_comp.v
@@ -2243,29 +2243,20 @@ econstructor.
     split. eapply MU.
   split. 
     split. eapply MU. clear MU.
-      destruct MTCH as [_ [_ [PG [_ [GF [SMV [WD _]]]]]]].
-      split. apply effstep_corestep in H.
-             eapply mem_respects_readonly_forward'. eassumption.
+      split.
+      apply effstep_corestep in H.
+             eapply mem_respects_readonly_fwd. eassumption.
              eapply corestep_fwd; eassumption.
-             eapply rtl_coop_readonly. apply H.
-         intros b GB. apply GF in GB. eapply SMV.
-         destruct (frgnSrc _ WD _ GB) as [bb [d [Frgn FTgt]]]. eapply foreign_DomRng; eassumption.
-     assert(G2: forall b, isGlobalBlock tge b = true -> Mem.valid_block m2 b).
-         rewrite <- (genvs_domain_eq_isGlobal _ _ GDE_lemma).
-         intros b GB. eapply SMV.
-         apply (meminj_preserves_globals_isGlobalBlock _ _ PG) in GB. 
-         eapply as_inj_DomRng; eassumption.
-     destruct CS2 as [CS2 | [CS2 _]]. 
-       apply effstep_plus_corestep_plus in CS2.
-             eapply mem_respects_readonly_forward'. eassumption.
+             eapply corestep_rdonly; eassumption.
+      destruct CS2 as [CS2 | [CS2 _]]. 
+        apply effstep_plus_corestep_plus in CS2.
+             eapply mem_respects_readonly_fwd. eassumption.
              eapply corestep_plus_fwd; eassumption.
-             eapply SM_simulation.CS2_RDO_plus; try eassumption.
-             apply rtl_coop_readonly. 
-       apply effstep_star_corestep_star in CS2.
-             eapply mem_respects_readonly_forward'. eassumption.
+             eapply corestep_plus_rdonly. eassumption. 
+      apply effstep_star_corestep_star in CS2.
+             eapply mem_respects_readonly_fwd. eassumption.
              eapply corestep_star_fwd; eassumption.
-             eapply SM_simulation.CS2_RDO_star; try eassumption.
-             apply rtl_coop_readonly. 
+             eapply corestep_star_rdonly. eassumption. 
   exists U2. split. assumption. intros. eapply MU. eassumption. }
 { (*halted*) 
   intros. destruct H as [[MC [RC [PG [GFP [GF [VAL [WD INJ]]]]]]] MRR]. 
