backend/Mach_coop.v
@@ -464,25 +464,10 @@ Lemma Mach_forward ge c m c' m': forall
       inv H0. eapply external_call_mem_forward; eassumption.
 Qed.
 
-Program Definition Mach_coop_sem : 
-  CoopCoreSem genv Mach_core.
-Proof.
-apply Build_CoopCoreSem with (coopsem := Mach_core_sem).
-  apply Mach_forward.
-Defined.
-
-End MACH_COOPSEM.
-
-Lemma mach_coop_readonly hf return_address_offset g c m c' m'
-            (CS: mach_step hf return_address_offset g c m c' m')
-            (GV: forall b, isGlobalBlock g b = true -> Mem.valid_block m b):  
-         RDOnly_fwd m m' (ReadOnlyBlocks g).
-  Proof. intros. red; intros.
-     unfold ReadOnlyBlocks in Hb.
-     remember (Genv.find_var_info g b) as d; symmetry in Heqd.
-     destruct d; try discriminate.
-     apply find_var_info_isGlobal in Heqd. apply GV in Heqd.  
-     (*destruct (MRR _ _ Heqd Hb) as [_ [VB _]].     *)
+Lemma mach_coop_readonly g c m c' m'
+            (CS: mach_step g c m c' m') b
+            (VB: Mem.valid_block m b): readonly m b m'.
+  Proof.
      inv CS; simpl in *; try apply readonly_refl.
           eapply store_stack_readonly; eassumption.
           destruct a; inv H0. eapply store_readonly; eassumption.
@@ -502,3 +487,13 @@ Lemma mach_coop_readonly hf return_address_offset g c m c' m'
               eapply store_stack_readonly; try eassumption. apply H1; apply H0; trivial.
           inv H0. eapply ec_readonly_strong; eassumption.
 Qed.
+
+Program Definition Mach_coop_sem : 
+  CoopCoreSem genv Mach_core.
+Proof.
+apply Build_CoopCoreSem with (coopsem := Mach_core_sem).
+  apply Mach_forward.
+  apply mach_coop_readonly.
+Defined.
+
+End MACH_COOPSEM.
