backend/Renumberproof_comp.v
@@ -1407,21 +1407,15 @@ Proof.
     split. eapply MU.
     split. 
       split. eapply MU. clear MU.
-      destruct MTCH as [_ [_ [PG [_ [GF [SMV [WD _]]]]]]].
-      split. apply effstep_corestep in H.
-             eapply mem_respects_readonly_forward'. eassumption.
+      split.
+      apply effstep_corestep in H.
+             eapply mem_respects_readonly_fwd. eassumption.
              eapply corestep_fwd; eassumption.
-             eapply rtl_coop_readonly. apply H.
-         intros b GB. apply GF in GB. eapply SMV.
-         destruct (frgnSrc _ WD _ GB) as [bb [d [Frgn FTgt]]]. eapply foreign_DomRng; eassumption.
+             eapply corestep_rdonly; eassumption.
       apply effstep_corestep in CS2.
-             eapply mem_respects_readonly_forward'. eassumption.
+             eapply mem_respects_readonly_fwd. eassumption.
              eapply corestep_fwd; eassumption.
-             eapply rtl_coop_readonly. apply CS2.
-         rewrite <- (genvs_domain_eq_isGlobal _ _ GDE_lemma).
-         intros b GB. eapply SMV.
-         apply (meminj_preserves_globals_isGlobalBlock _ _ PG) in GB. 
-         eapply as_inj_DomRng; eassumption.
+             eapply corestep_rdonly; eassumption.
     exists U2. split. left. apply effstep_plus_one. trivial.
   eapply MU. }
 Qed.
