cfrontend/Clight_self_simulates.v
@@ -3698,23 +3698,15 @@ intros.
     split. eapply HU.
     split.
       split. eapply HU. clear HU.
-      destruct MTCH as [_ [_ [PG [GF [SMV WD]]]]].
-      split. apply effstep_corestep in H.
-             eapply (mem_respects_readonly_forward' _ m1). eassumption.
+      split.
+      apply effstep_corestep in H.
+             eapply (mem_respects_readonly_fwd _ m1). eassumption.
              eapply corestep_fwd; eassumption.
-             eapply clight1_coop_readonly. apply H.
-         intros b GB. apply GF in GB. eapply SMV.
-         destruct (frgnSrc _ WD _ GB) as [bb [d [Frgn FTgt]]]. eapply foreign_DomRng; eassumption.
-     assert(G2: forall b, isGlobalBlock tge b = true -> Mem.valid_block m2 b).
-         rewrite <- (genvs_domain_eq_isGlobal _ _ GDE_lemma).
-         intros b GB. eapply SMV.
-         apply (meminj_preserves_globals_isGlobalBlock _ _ PG) in GB. 
-         eapply as_inj_DomRng; eassumption.
-     apply effstep_plus_corestep_plus in CS2.
-             eapply mem_respects_readonly_forward'. eassumption.
+             eapply corestep_rdonly; eassumption.
+        apply effstep_plus_corestep_plus in CS2.
+             eapply (mem_respects_readonly_fwd _ m2). eassumption.
              eapply corestep_plus_fwd; eassumption.
-             eapply SM_simulation.CS2_RDO_plus; try eassumption.
-             apply clight1_coop_readonly. 
+             eapply corestep_plus_rdonly. eassumption. 
     exists U2. split. left; assumption. apply HU. }
 Qed.
 
