core/semantics_lemmas.v
@@ -164,4 +164,31 @@ Proof.
    apply H.
 Qed.
 
+Lemma corestepN_rdonly: forall ge c m c' m' n,
+  corestepN coopsem ge n c m c' m' -> forall b
+  (VB: Mem.valid_block m b), readonly m b m'.
+Proof.
+intros until n; revert c m.
+induction n; simpl; auto.
+inversion 1; intros. apply readonly_refl.
+intros c m [c2 [m2 [? ?]]].
+intros. apply readonly_trans with (m2 := m2).
+eapply corestep_rdonly; eauto.
+eapply IHn; eauto. eapply corestep_fwd; eauto.
+Qed.
+
+Lemma corestep_plus_rdonly ge c m c' m'
+  (CS: corestep_plus coopsem ge c m c' m') b
+  (VB: Mem.valid_block m b): readonly m b m'.
+Proof.
+  destruct CS. eapply corestepN_rdonly; eauto. 
+Qed.
+
+Lemma corestep_star_rdonly ge c m c' m'
+  (CS: corestep_star coopsem ge c m c' m') b
+  (VB: Mem.valid_block m b): readonly m b m'.
+Proof.
+  destruct CS. eapply corestepN_rdonly; eauto. 
+Qed.
+
 End CoopCoreSemLemmas.
